MachCSL/WpSmodeTrapCsr.lean
@@ -439,7 +439,7 @@ theorem execSpecF_csrw_sstatus_off (cpu : CPU) (c : MConf) (sie : Bool) (hok : S
   swp_run 80
   ihave HmConf := confCells_intro _ _ _ { c with mstatus := sstatusWrite c.mstatus (R.get rs1) } $$ [Hcur_privilege Hhart_state Hmisa Hmstatus Hmie
     Hmideleg Hmedeleg Hmepc Hsatp Hmenvcfg Hmcounteren Hscounteren Hmtimecmp Hstimecmp Hpmpcfg_n
-    Hpmpaddr_n Hsig_meip Hsig_seip Hmseccfg Help Hsenvcfg Hmcountinhibit Hminstretcfg
+    Hpmpaddr_n Hmseccfg Help Hsenvcfg Hmcountinhibit Hminstretcfg
     Hmcyclecfg Hpma_regions Hhtif_tohost_base]
   case' _ => iframe
   iapply HΦ $$ HmConf HPC HnextPC HF
