MachCSL/WpSmodeWait.lean
@@ -55,8 +55,6 @@ def confCellsHS (cpu : CPU) (dq : DFrac) (p : Privilege) (c : MConf) (hs : HartS
   Register.stimecmp ↦ᵣ[cpu]{dq} c.stimecmp ∗
   Register.pmpcfg_n ↦ᵣ[cpu]{dq} c.pmpcfg ∗
   Register.pmpaddr_n ↦ᵣ[cpu]{dq} c.pmpaddr ∗
-  Register.sig_meip ↦ᵣ[cpu]{dq} 0#1 ∗
-  Register.sig_seip ↦ᵣ[cpu]{dq} 0#1 ∗
   Register.mseccfg ↦ᵣ[cpu]{dq} 0#64 ∗
   Register.elp ↦ᵣ[cpu]{dq} 0#1 ∗
   Register.senvcfg ↦ᵣ[cpu]{dq} 0#64 ∗
@@ -88,8 +86,6 @@ theorem confCellsHS_cases (cpu : CPU) (dq : DFrac) (p : Privilege) (c : MConf) (
     Register.stimecmp ↦ᵣ[cpu]{dq} c.stimecmp ∗
     Register.pmpcfg_n ↦ᵣ[cpu]{dq} c.pmpcfg ∗
     Register.pmpaddr_n ↦ᵣ[cpu]{dq} c.pmpaddr ∗
-    Register.sig_meip ↦ᵣ[cpu]{dq} 0#1 ∗
-    Register.sig_seip ↦ᵣ[cpu]{dq} 0#1 ∗
     Register.mseccfg ↦ᵣ[cpu]{dq} 0#64 ∗
     Register.elp ↦ᵣ[cpu]{dq} 0#1 ∗
     Register.senvcfg ↦ᵣ[cpu]{dq} 0#64 ∗
@@ -117,8 +113,6 @@ theorem confCellsHS_intro (cpu : CPU) (dq : DFrac) (p : Privilege) (c : MConf) (
     Register.stimecmp ↦ᵣ[cpu]{dq} c.stimecmp ∗
     Register.pmpcfg_n ↦ᵣ[cpu]{dq} c.pmpcfg ∗
     Register.pmpaddr_n ↦ᵣ[cpu]{dq} c.pmpaddr ∗
-    Register.sig_meip ↦ᵣ[cpu]{dq} 0#1 ∗
-    Register.sig_seip ↦ᵣ[cpu]{dq} 0#1 ∗
     Register.mseccfg ↦ᵣ[cpu]{dq} 0#64 ∗
     Register.elp ↦ᵣ[cpu]{dq} 0#1 ∗
     Register.senvcfg ↦ᵣ[cpu]{dq} 0#64 ∗
@@ -136,7 +130,7 @@ set_option hygiene false in
 macro "confhs_cases " h:ident : tactic =>
   `(tactic| ihave ⟨Hcur_privilege, Hhart_state, Hmisa, Hmstatus, Hmie, Hmideleg, Hmedeleg, Hmepc,
                   Hsatp, Hmenvcfg, Hmcounteren, Hscounteren, Hmtimecmp, Hstimecmp, Hpmpcfg_n, Hpmpaddr_n,
-                  Hsig_meip, Hsig_seip, Hmseccfg, Help, Hsenvcfg, Hmcountinhibit, Hminstretcfg,
+                  Hmseccfg, Help, Hsenvcfg, Hmcountinhibit, Hminstretcfg,
                   Hmcyclecfg, Hpma_regions, Hhtif_tohost_base⟩ := confCellsHS_cases _ _ _ _ _ $$ $h:ident)
 
 open Iris.ProofMode in
@@ -145,7 +139,7 @@ set_option hygiene false in
 macro "confhs_intro " h:ident : tactic =>
   `(tactic| (ihave $h:ident := confCellsHS_intro _ _ _ _ _ $$ [Hcur_privilege Hhart_state Hmisa Hmstatus Hmie
                   Hmideleg Hmedeleg Hmepc Hsatp Hmenvcfg Hmcounteren Hscounteren Hmtimecmp Hstimecmp Hpmpcfg_n
-                  Hpmpaddr_n Hsig_meip Hsig_seip Hmseccfg Help Hsenvcfg Hmcountinhibit Hminstretcfg
+                  Hpmpaddr_n Hmseccfg Help Hsenvcfg Hmcountinhibit Hminstretcfg
                   Hmcyclecfg Hpma_regions Hhtif_tohost_base]
              case' _ => iframe))
 
